RiddleProofs.lean
@@ -1,4 +1,3 @@
-import RiddleProofs.BlueEyedIslanders
 import RiddleProofs.JealousHusbands
 import RiddleProofs.MontyHall
 import RiddleProofs.LightsOut
